Progress, stuck on  Let (Coq proof of correctness)

cogent/llvm/checker/coq/Correctness.v
@@ -6,14 +6,17 @@ From Vellvm Require Import LLVMAst LLVMEvents TopLevel Handlers InterpreterMCFG 
   DynamicValues ExpLemmas Coqlib NoFailure AListFacts.
 
 From Checker Require Import Denotation DenotationTheory Cogent Compiler Utils.Tactics Invariants
-  HelixLib.Correctness_Prelude HelixLib.BidBound HelixLib.IdLemmas HelixLib.VariableBinding Types.
+  HelixLib.Correctness_Prelude HelixLib.BidBound HelixLib.IdLemmas HelixLib.VariableBinding Types
+HelixLib.StateCounters.
 
 Import ListNotations.
 Import AlistNotations.
 
 Import ExpTactics.
 Import ProofMode.
+Import LidBound.
 
+(* The following sections should be put in the relevant files in HelixLib/ *)
 Section BidBoundExtra.
 
   (* From Helix, but adjusted for Cogent - are these definitely still true? *)
@@ -59,6 +62,219 @@ Section BidBoundExtra.
 
 End BidBoundExtra.
 
+Section InvariantExtra.
+Definition gamma_bound (s : IRState) : Prop :=
+  forall n id τ,
+    nth_error (Γ s) n ≡ Some (τ, EXP_Ident (ID_Local id)) ->
+    lid_bound s id.
+
+Lemma in_gamma_not_in_neq :
+  forall σ s id r,
+    in_Gamma σ s id ->
+    ~ in_Gamma σ s r ->
+    id ≢ r.
+Proof.
+  intros σ s id r GAM NGAM.
+  destruct (Eqv.eqv_dec_p r id) as [EQ | NEQ].
+  - do 2 red in EQ.
+    subst.
+    contradiction.
+  - unfold Eqv.eqv, eqv_raw_id in NEQ.
+    eauto.
+Qed.
+(* TODO: move this? *)
+Lemma incLocal_id_neq :
+  forall s1 s2 s3 s4 id1 id2,
+    incLocal s1 ≡ inr (s2, id1) ->
+    incLocal s3 ≡ inr (s4, id2) ->
+    local_count s1 ≢ local_count s3 ->
+    id1 ≢ id2.
+Proof.
+Admitted.
+
+Lemma incBlockNamed_id_neq :
+  forall s1 s2 s3 s4 id1 id2 n1 n2,
+    incBlockNamed n1 s1 ≡ inr (s2, id1) ->
+    incBlockNamed n2 s3 ≡ inr (s4, id2) ->
+    is_correct_prefix n1 ->
+    is_correct_prefix n2 ->
+    block_count s1 ≢ block_count s3 ->
+    id1 ≢ id2.
+Proof.
+  intros s1 s2 s3 s4 id1 id2 n1 n2 GEN1 GEN2 PRE1 PRE2 COUNT.
+  eapply incBlockNamed_count_gen_injective; eauto.
+Qed.
+
+
+(*
+Ltac solve_id_neq :=
+  first [ solve [eapply incLocal_id_neq; eauto; solve_local_count]
+        | solve [eapply incBlockNamed_id_neq; eauto; solve_block_count]
+        | solve [eapply in_gamma_not_in_neq; [solve_in_gamma | solve_not_in_gamma]]
+        | solve [eapply lid_bound_earlier; [ solve_lid_bound | solve_lid_bound_between  | solve_local_count ]]
+        | solve [eapply state_bound_between_separate; [eapply incLocalNamed_count_gen_injective
+                                                      | solve_lid_bound_between
+                                                      | solve_lid_bound_between
+                                                      | cbn; solve_local_count]]
+        | solve [let CONTRA := fresh "CONTRA" in intros CONTRA; symmetry in CONTRA; revert CONTRA; solve_id_neq]
+        ].
+*)
+Lemma state_invariant_escape_scope:
+  ∀ (σ : list _) v x (s1 s2 : IRState) stH 
+    (stV : config_cfg),
+    Γ s1 ≡ x :: Γ s2 → gamma_bound s2 → state_invariant (v :: σ) s1 stH stV → state_invariant σ s2 stH stV.
+  Admitted.
+
+Lemma lid_bound_between_shrink_up:
+  ∀ (s1 s2 s3 : IRState) (id : local_id), s2 <<= s3 → lid_bound_between s1 s2 id → lid_bound_between s1 s3 id.
+  Admitted.
+Lemma lid_bound_between_shrink_down:
+  ∀ (s1 s2 s3 : IRState) (id : local_id), s1 <<= s2 → lid_bound_between s2 s3 id → lid_bound_between s1 s3 id.
+  Admitted.
+Lemma lid_bound_between_shrink:
+  ∀ (s1 s2 s3 s4 : IRState) (id : local_id),
+    lid_bound_between s2 s3 id → s1 <<= s2 → s3 <<= s4 → lid_bound_between s1 s4 id.
+  Admitted.
+
+(* This lemma is not in helix *)
+Lemma local_scope_preserved_mono pre_state mid_state post_state l1 l2 :
+  pre_state <<= mid_state -> 
+  mid_state <<= post_state -> 
+  local_scope_preserved pre_state post_state l1 l2 
+  -> local_scope_preserved mid_state post_state l1 l2.
+  intros le_pre le_mid h id hid.
+  apply h.
+  eapply lid_bound_between_shrink_down; eassumption.
+Qed.
+
+  (* Given a range defined by [s1;s2], ensures that the whole range is irrelevant to the memory invariant *)
+  Definition Gamma_safe σ (s1 s2 : IRState) : Prop :=
+    forall id, lid_bound_between s1 s2 id ->
+               ~ in_Gamma σ s1 id.
+
+  Lemma Gamma_preserved_if_safe:
+  ∀ (σ : ctx) (s1 s2 : IRState) (l1 l2 : local_env),
+    Gamma_safe σ s1 s2 → local_scope_modif s1 s2 l1 l2 → Gamma_preserved σ s1 l1 l2.
+Admitted.
+
+  (* is it really true? *)
+  Lemma Gamma_safe_Context_extend:
+  ∀ (σ : ctx) (s1 s2 : IRState),
+    Gamma_safe σ s1 s2
+    → ∀ (s1' s2' : IRState) (x : raw_id) (v : typ) (xτ : _ ),
+        s1 <<= s1'
+        → local_count s2 ≥ local_count s2'
+          → Γ s1' ≡ (v, EXP_Ident (ID_Local x)) :: Γ s1
+            → Γ s2' ≡ (v, EXP_Ident (ID_Local x)) :: Γ s2
+              → (∀ id : local_id, lid_bound_between s1' s2' id → x ≢ id) → Gamma_safe (xτ :: σ) s1' s2'.
+  Admitted.
+
+  Lemma Gamma_safe_Context_extend':
+  ∀ (σ : ctx) (s1 s2 : IRState),
+    Gamma_safe σ s1 s2
+    → ∀ (s1' s2' : IRState) y  (xτ : _ ),
+        s1 <<= s1'
+        → local_count s2 ≥ local_count s2'
+          → Γ s1' ≡ y :: Γ s1
+            → Γ s2' ≡ y :: Γ s2
+            -> (forall (x : raw_id)(v : typ), y ≡ (v, EXP_Ident (ID_Local x)) ->
+                                        (∀ id : local_id, lid_bound_between s1' s2' id → x ≢ id)
+              )
+              → Gamma_safe (xτ :: σ) s1' s2'.
+    intros ??? safe .
+    intros .
+    intros ?? h.  
+    inversion h; subst; cbn in *.
+
+    rewrite H1 in H6.
+    destruct n; revgoals; cbn in *.
+    - unfold Gamma_safe in safe.
+      unfold not in safe.
+      eapply safe.
+      eapply lid_bound_between_shrink; eassumption.
+      econstructor; eassumption.
+    - destruct y as [ y w ].
+      injection H6.
+      intros hw hy.
+
+      destruct w; try discriminate.
+      subst .
+      injection hw.
+      intro; subst id0.
+      eapply Gamma_safe_Context_extend; try eassumption.
+      eapply H3.
+      reflexivity.
+    Qed.
+
+  (* Not in Helix because not needed there *)
+  Lemma Gamma_preserved_Context_extend:
+  ∀ (σ : ctx) (s1 s2 : IRState)xτ l1 l2 y,
+    Gamma_preserved σ s1 l1 l2 ->
+          Γ s2 ≡ y :: Γ s1
+            -> (forall (x : raw_id)(v : typ), y ≡ (v, EXP_Ident (ID_Local x)) -> l1 @ x ≡ l2 @ x)
+              
+              -> Gamma_preserved (xτ :: σ) s2 l1 l2.
+    Proof.
+      intros * Gp eqG eqid.
+      unfold Gamma_preserved.
+      intro id.
+      intro h.
+      inversion h; subst; cbn in *.
+      rewrite eqG in H0.
+      destruct n; revgoals; cbn in *.
+      - eapply Gp.
+        econstructor; eassumption.
+      - destruct y as [ y w ].
+        injection H0.
+        intros hw hy.
+        destruct w; try discriminate.
+        subst .
+        injection hw.
+        intro; subst id0.
+        eapply eqid.
+        reflexivity.
+    Qed.
+
+Lemma Gamma_safe_shrink:
+  ∀ (σ : ctx) (s1 s2 s3 s4 : IRState),
+    Gamma_safe σ s1 s4 → Γ s1 ≡ Γ s2 → s1 <<= s2 → s3 <<= s4 → Gamma_safe σ s2 s3.
+  Admitted.
+
+Lemma local_scope_modif_trans:
+  ∀ (s1 s2 s3 : IRState) (l1 l2 l3 : local_env),
+    s1 <<= s2
+    → s2 <<= s3 → local_scope_modif s1 s2 l1 l2 → local_scope_modif s2 s3 l2 l3 → local_scope_modif s1 s3 l1 l3.
+  Admitted.
+
+Lemma st_gamma_bound:
+  ∀ (σ : ctx) (s : IRState) (memH : _) (configV : config_cfg),
+    state_invariant σ s memH configV → gamma_bound s.
+Admitted.
+Lemma gamma_bound_mono: ∀ s1 s2 : IRState, gamma_bound s1 → s1 <<= s2 → Γ s1 ≡ Γ s2 → gamma_bound s2.
+Admitted.
+End InvariantExtra.
+
+
+Section ContextExtra.
+
+Lemma compile_expr_Γ :
+ ∀ (op : Cogent.expr) (s1 s2 : IRState) (nextblock b : block_id) (bk_op : list (LLVMAst.block typ)) r,
+  compile_expr op nextblock s1 ≡ inr (s2, (r, b, bk_op)) → Γ s1 ≡ Γ s2.
+Admitted.
+
+End ContextExtra.
+
+Section Correctness_NExpr_Extra.
+(* originally: genNExpr_ident_bound *)
+Lemma compile_expr_ident_bound :
+  ∀ (nexp : Cogent.expr) (s1 s2 : IRState) b (id : raw_id) t  bentry c,
+    compile_expr nexp b s1 ≡ inr (s2, ((t, EXP_Ident (ID_Local id)), bentry, c)) → gamma_bound s1 → lid_bound s2 id.
+Admitted.
+End Correctness_NExpr_Extra.
+
+
+
+
 Section Block.
 
   (* wasn't sure how to do this rewrite *)
@@ -82,6 +298,7 @@ Section Expressions.
   Definition compile_expr_post (i : im) (γ : ctx) (s1 s2 : IRState) (to : block_id)
                                (l : local_env) : Rel_cfg_T uval ocfg_res :=
     lift_Rel_cfg (state_invariant γ s2) ⩕
+    (* inspired by genNExpr_post *)
     correct_result_T γ s1 s2 i ⩕
     branches to ⩕
     (fun _ '(_, (l', _)) => local_scope_modif s1 s2 l l').
@@ -124,12 +341,13 @@ Section Expressions.
       no_failure (interp_expr (E := E_cfg) (denote_expr γ e) memC) ->
       bid_bound s1 next_bid ->
       state_invariant γ s1 memC (memV, (l, g)) ->
+      Gamma_safe γ s1 s2 ->
       eutt
         (succ_cfg (compile_expr_post v γ s1 s2 next_bid l))
         (interp_expr (denote_expr γ e) memC)
         (interp_cfg (denote_ocfg (convert_typ [] blks) (prev_bid, entry_bid)) g l memV).
   Proof.
-    induction e using expr_ind'; intros * COMP NOFAIL NEXT PRE.
+    induction e using expr_ind'; intros * COMP NOFAIL NEXT PRE GAM.
     - (* Unit *)
       cbn* in *; simp.
       cbn*.
@@ -177,14 +395,22 @@ Section Expressions.
       contradiction.
       apply find_block_nil.
     - (* Let e1 e2 *)
-      pose proof COMP as COMP'.
-      cbn* in COMP'; simp.
+      cbn* in COMP.
+      simp.
       rename s1 into pre_state, i into mid_state, i1 into post_state.
       rename l0 into e1_blks, l1 into e2_blks.
       rename b0 into e2_entry, entry_bid into e1_entry.
       rename t into e1_im_t, e into e1_im, t0 into e2_im_t, e0 into e2_im.
       rename t1 into new_var, l2 into cur_vars.
       rename Heqs into COMP_e1, Heqs1 into COMP_e2, Heql3 into BIND.
+      assert (Γeq := COMP_e2).
+      apply compile_expr_Γ in Γeq.
+      cbn in Γeq.
+      rewrite BIND in Γeq.
+      injection Γeq.
+      intros ??; subst cur_vars new_var.
+      clear Γeq.
+
       cbn.
       clean_goal.
 
@@ -217,8 +443,9 @@ Section Expressions.
         apply incBlockNamed_count_gen_mono.
         eassumption.
         eassumption.
-        solve_block_count.
-        solve_block_count.
+        reflexivity.
+        cbn.
+        auto.
       }
       cvred.
       cbn in *.
@@ -229,6 +456,9 @@ Section Expressions.
         - eapply no_failure_expr_bind_prefix; exact NOFAIL.
         - eapply bid_bound_incBlockNamed with (name := "Let"); solve_prefix.
         - apply state_invariant_new_block; assumption.
+        - eapply Gamma_safe_shrink; eauto.
+          cbn.
+          solve_local_count.
       }
       clear IHe1.
       introR.
@@ -243,48 +473,280 @@ Section Expressions.
       apply find_block_eq; auto.
       repeat vred.
       rewrite (cons_app _ (convert_typ [] e2_blks)).
-      rewrite denote_ocfg_app_no_edges.
-      3: {
-        unfold no_reentrance.
-        simpl.
-        eapply Forall_disjoint.
-        apply outputs_bound_between in COMP_e2.
-        exact COMP_e2.
-        apply Forall_cons; auto.
-        eapply bid_bound_incBlockNamed with (name := "Let"); solve_prefix.
-        cbn.
-        admit. (* TODO: Doesn't look true - this is a bit different to how it was above *)
+      set (let_bid := ("Let" @@ string_of_nat (block_count pre_state))) in *.
+      assert (Let_bid_bond :   bid_bound
+                                 {|
+                                   block_count := S (block_count pre_state);
+                                   local_count := local_count pre_state;
+                                   void_count := void_count pre_state;
+                                   Γ := Γ pre_state |} let_bid).
+      {
+        apply bid_bound_incBlockNamed with (name := "Let") (s1 := pre_state).
+        solve_prefix.
+        reflexivity.
       }
+      assert(Let_bid_bond_mid :
+               bid_bound
+                 {|
+                   block_count := block_count mid_state;
+                   local_count := local_count mid_state;
+                   void_count := void_count mid_state;
+                   Γ := (e1_im_t, e1_im) :: Γ mid_state |} let_bid
+            ).
+      {
+        
+        eapply bid_bound_mono.
+        + exact Let_bid_bond. 
+        + solve_block_count. 
+      }           
+      assert(neq_let_next_bid : Name let_bid ≢ next_bid).
+      {
+        
+        intro.
+        subst next_bid.
+        apply bid_bound_name in NEXT.
+        revert NEXT.
+        lia.
+        solve_prefix.
+      }
+
+      (* like helix/Correctness_GenIR *)
+      rewrite denote_ocfg_app; eauto.
       2: {
+        unfold no_reentrance.
+        assert (GEN_OP1 := COMP_e1).
+        assert (GEN_OP2 := COMP_e2).
+        pose proof GEN_OP1 as GEN_OP1'.
+        pose proof GEN_OP2 as GEN_OP2'.
+        
+        apply (inputs_not_earlier_bound _ _ _ _ _ _ _ _ _ NEXT) in GEN_OP1'.
+        apply (inputs_not_earlier_bound _ _ _ _ _ _ _ _ _ NEXT) in GEN_OP2'.
+        apply inputs_bound_between in GEN_OP1.
+        apply outputs_bound_between in GEN_OP2.
+
+        pose proof (Forall_and GEN_OP1 GEN_OP1') as INPUTS.
+        cbn in INPUTS.
         cbn.
-        apply entry_bound_between in COMP_e2.
-        destruct COMP_e2 as [OUT_PRED | OUT_PRED].
-        - admit. (* TODO: because e2_entry bound after mid_state, can't be = pre_state *)
-        - admit. (* TODO: becayse e2_entry = next_bid, can't be pre_state *)
+        
+
+        apply list_disjoint_singleton_right.
+        intro hin.
+        rewrite Forall_forall in GEN_OP2.
+        specialize (GEN_OP2 _ hin).
+        revert GEN_OP2.
+        intro OUT_PRED .
+        cbn in OUT_PRED.
+        destruct OUT_PRED as [OUT_PRED | OUT_PRED]; revgoals.
+        revert OUT_PRED; exact neq_let_next_bid.
+        revert OUT_PRED.
+        eapply not_bid_bound_between.
+        assumption.
+        solve_block_count.
+        solve_block_count.
       }
+      
+
+      
+      rewrite interp_cfg3_bind.
+      rewrite denote_ocfg_unfold_not_in; revgoals.
+        {
+          cbn.
+          rewrite find_block_ineq.
+          reflexivity.
+          cbn.
+          intro heq.
+          subst e2_entry.
+          apply entry_bound_between in COMP_e2.
+          case COMP_e2.
+          - apply not_bid_bound_between.
+            assumption.
+          - assumption.
+        }
+        vred.
+
+        assert (Gamma_safe_mid_post :
+                  Gamma_safe (vC :: γ)
+                             {|
+                               block_count := block_count mid_state;
+                               local_count := local_count mid_state;
+                               void_count := void_count mid_state;
+                               Γ := (e1_im_t, e1_im) :: Γ mid_state |} post_state
+               ).
+        {
+            eapply Gamma_safe_Context_extend'; eauto.
+            cbn.
+            solve_local_count.
+            cbn.
+            f_equal.
+            assert (h1 := COMP_e1).
+            apply compile_expr_Γ in h1.
+            revert h1.
+            cbn.
+            auto.
+            intros x v eq.
+            injection eq.
+            intros ??; subst v.
+            subst e1_im.
+            rename x into e1_im.
+            cbn.
+            intros id h.
+            (* following Helix/Correct_Alloc *)
+            revert h.
+            eapply lid_bound_fresh; eauto.
+            eapply compile_expr_ident_bound in COMP_e1.
+            exact COMP_e1.
+            eapply gamma_bound_mono.
+            eapply st_gamma_bound.
+            exact PRE.
+            cbn.
+            reflexivity.
+            reflexivity.
+        }
+        assert (INV_mid_ext :
+                  state_invariant
+                    (vC :: γ)
+                    {|
+                      block_count := block_count mid_state;
+                      local_count := local_count mid_state;
+                      void_count := void_count mid_state;
+                      Γ := (e1_im_t, e1_im) :: Γ mid_state |}
+                    memH (memV0, (l0, g0))
+               ).
+        {
+          (* probably apply some Lemma similar to Helix' state_invariant_enter_scope_* *)
+            admit. (* TODO: prove state_invariant s => state_invariant with new variable *)
+        }
+
+        eassert (IHe2'' :
+                   eutt
+                     _
+                     (interp_expr (denote_expr (_ :: γ) e2) _)
+                     (interp_cfg3(denote_ocfg (convert_typ [] _) (_, _))
+                                 g0 l0 memV0
+                     )
+).
+        {
+          apply (IHe2 (_ :: γ)).
+          * exact COMP_e2.
+          * exact NOFAIL.
+          * cbn.
+            eapply bid_bound_mono.
+            -- exact NEXT.
+            -- cbn.
+               solve_block_count.
+          * cbn.
+            exact INV_mid_ext.
+          * exact Gamma_safe_mid_post.
+        }
+
+     assert(Gamma_bound_mid_post :
+                   gamma_bound
+    {|
+    block_count := block_count post_state;
+    local_count := local_count post_state;
+    void_count := void_count post_state;
+    Γ := Γ mid_state |}
+           ).
+     {
+       eapply gamma_bound_mono.
+       eapply st_gamma_bound.
+       exact INV2.
+       cbn.
+       solve_local_count.
+       reflexivity.
+     }
 
       (* last blocks *)
       eapply eqit_mon; auto.
-      2: {
-        eapply IHe2.
-        exact COMP_e2.
-        auto.
-        eapply bid_bound_mono.
-        eassumption.
-        cbn.
-        admit. (* TODO: prove bid_bound pre_state => bid_bound mid_state *)
-        admit. (* TODO: prove state_invariant s => state_invariant with new variable *)
-      }
-      clear IHe2.
+      2: exact IHe2''. 
+      clear IHe2 IHe2''.
       intros [[memC1 ?]|] (memV1 & l1 & g1 & res1) PR; [| inv PR].
       destruct PR as [S1 [C1 [B1 L1]]].
       cbn in S1.
-      split; cbn.
-      admit. (* TODO: state_invariant *)
-      split; cbn.
-      admit. (* TODO: correct result *)
-      split; auto.
-      admit. (* TODO: local scope modif *)
+      split; [| split]; [| |  split]; cbn ;eauto.
+      + cbn.
+        revert S1.
+        eapply state_invariant_escape_scope.
+        exact BIND.
+        cbn.
+        exact Gamma_bound_mid_post.
+      + intros.
+        cbn in C1.
+        rewrite C1.
+        reflexivity.
+        all:clear C1.
+        * eapply local_scope_preserved_mono; revgoals; cbn.
+           exact H.
+          -- apply compile_expr_local_count in COMP_e2.
+             exact COMP_e2.
+          -- apply compile_expr_local_count in COMP_e1.
+             exact COMP_e1.
+        * cbn.
+(* I currently don't know how to prove this goal.
+In Helix, they use some tactic solve_gamma_preserved:
+
+Hint Immediate Gamma_preserved_refl : SolveGammaPreserved.
+Hint Extern 1 (~ (in_Gamma _ _ _)) => solve_not_in_gamma : SolveGammaPreserved.
+Hint Resolve Gamma_preserved_add_not_in_Gamma : SolveGammaPreserved.
+Hint Resolve Gamma_preserved_if_safe : SolveGammaPreserved.
+Hint Extern 1 (local_scope_modif _ _ _ _) => solve_local_scope_modif : SolveGammaPreserved.
+Hint Extern 1 (Gamma_safe _ _ _) => solve_gamma_safe : SolveGammaPreserved.
+
+Ltac solve_gamma_preserved :=
+  solve [eauto with SolveGammaPreserved].
+
+ *)
+          (*
+
+If the identifier e1_im was explicitly created for the variable in the
+Let case, would it be work better?
+*)
+          eapply Gamma_preserved_Context_extend.
+          eassumption.
+          cbn.
+          apply compile_expr_Γ in COMP_e1; cbn in COMP_e1; rewrite COMP_e1.
+          reflexivity.
+          intros x v eq.
+          injection eq.
+          intros ??; subst v.
+          subst e1_im.
+          rename x into e1_im.
+          Search e1_im.
+(* In Helix, γ only contains identifiers, rather than expressions. 
+   (this is an optimisation in case the variable's value is a constant) *)
+
+          (* here I work on hypothesis S1, but I am not sure it is useful *)
+          apply mem_is_inv in S1.
+          red in S1.
+          specialize (S1 (O : nat)).
+          rewrite BIND in S1.
+          specialize (S1 _ _ eq_refl eq_refl).
+          cbn in S1.
+
+          (* I am tempted to apply hypothesis H *)
+          symmetry.
+          apply H.
+          assert (he1 := COMP_e1).
+          eapply compile_expr_ident_bound in he1.
+          revert he1.
+          Search e1_im.
+          (*
+I think lid_bound mid_state e1_im (the last reverted assumption) implies either
+1) either lid_bound pre_state,
+2) either lid_bound_between pre_state mid_state
+
+2) easily implies the goal, but 1) is contradicts the goal...
+So, why 1) is false? Maybe it was a wrong to apply H.
+           *)
+          revert COMP_e1.
+          admit.
+          eapply st_gamma_bound.
+          eapply state_invariant_new_block.
+          eassumption.
+      + revert POST L1.
+        apply compile_expr_local_count in COMP_e1.
+        apply compile_expr_local_count in COMP_e2.
+        eapply (@local_scope_modif_trans pre_state mid_state post_state); eassumption.
     - (* Prim op os *)
       cbn* in *; simp.
       admit.
@@ -344,6 +806,7 @@ Section Expressions.
           exact NOFAIL.
         - eapply bid_bound_incBlockNamed with (name := "Field"); solve_prefix.
         - apply state_invariant_new_block; assumption.
+        - admit. (* TODO: gamma safe *)
       }
       clear IHe.
       introR.
@@ -437,6 +900,7 @@ Section Expressions.
         reflexivity.
         apply state_invariant_new_block.
         assumption.
+        admit. (* TODO: Gamma_safe *)
       }
       clear IH_arg.
       introR.
@@ -466,6 +930,7 @@ Section TopLevel.
   (* placeholder *)
   Definition R {A B} (x: A) (y: B):= True.
 
+  (* Correctness_NExpr describes some tactics *)
   Theorem compiler_correct :
     forall (c : cogent_prog) (ll : vellvm_prog),
       compile_cogent c ≡ inr ll ->
